Move Automaton module into separate file. see #32

src/dafny/CFGBuilder/BuildCFGSimplified.dfy
@@ -14,117 +14,13 @@
 
 include "../utils/MiscTypes.dfy"
 include "../utils/int.dfy"
+include "../utils/AutomataV2.dfy" 
 
 module DFSSimple {
 
-  import opened MiscTypes
+  import opened MiscTypes 
   import opened Int
-
-  function FunctionByMethodTailRecursion(x: int, y: int := 0): (r: int) {
-    x + y
-  } by method {
-    if x < 8 || x == 77 {
-      return x + y;
-    } else {
-      r := FunctionByMethodTailRecursion(x - 1, y + 1);
-    }
-  }
-
-  datatype Graph<!T(==)> = Graph(init: T, succ: T -> seq<T>)
-
-  datatype Auto<!T(!new,==)> = Auto(toString: T -> string, transitions: map<T, seq<T>> := map[], states: seq<T> := [])
-  {
-    function addEdge(i: T, j: T): (a: Auto<T>)
-      requires IsValid()
-      ensures a.IsValid()
-    {
-      if i in transitions then
-        if j in transitions[i] then
-          this
-        else
-          this
-          .(transitions := transitions[i := transitions[i] + [j]] + (if j !in states then map[j := []] else map[]))
-          .(states  := states + (if j in states then [] else [j]))
-      else
-        this
-        .(transitions := transitions + map[i := [j]] + map[j := []])
-        .(states := states + [i, j])
-    }
-
-    /**
-      * Returns the number of states of the automaton.
-      */
-    function SSize(): nat
-      requires this.IsValid()
-    {
-      |states|
-    }
-
-    /** Number of transitions of the automaton. */
-    function TSize(xd: seq<T> := states): nat
-      requires this.IsValid()
-      requires (forall i : T :: i in xd ==> i in transitions)
-    {
-      if xd == [] then 0
-      else
-        assert xd[0] in states;
-        |transitions[xd[0]]| + TSize(xd[1..])
-    }
-
-    /**
-      * String representation of a state.
-      */
-    function ToString(t: T): string {
-      toString(t)
-    }
-
-    /** Print to Dot format. */
-    method {:print} ToDot()
-      requires this.IsValid()
-    {
-      print "digraph G {\n";
-      print "// Number of states: ", NatToString(SSize()), "\n";
-      print "// Number of transitions : ", NatToString(TSize()), "\n";
-      for i := 0 to |states| {
-        print ToString(states[i]) + ";\n";
-      }
-      for i := 0 to |states| {
-        for j := 0 to |transitions[states[i]]| {
-          print ToString(states[i]) + " -> " + ToString(transitions[states[i]][j]) +
-                "[label=\"" + NatToString(j) + "\"]"
-                + ";\n";
-        }
-      }
-      print "}\n";
-    }
-
-    ghost predicate IsValid() {
-      && (forall i : T :: i in states <==> i in transitions)
-    }
-  }
-
-  /** Attempt at defining a constraint on functions  */
-  type WellDefined<!K(!new)> =
-    f: (K, seq<K>) -> Option<K> | (forall x: K, xs: seq<K> {:triggers f(x, xs)} :: f(x, xs).Some? ==> f(x, xs).v in xs)
-    witness ( (x: K, xs: seq<K>) => None)
-
-  type WellDefined2<!K(!new)> =
-    f: (K, seq<K>) -> Option<nat> | (forall x: K, xs: seq<K> {:triggers f(x, xs)} :: f(x, xs).Some? ==> f(x, xs).v < |xs|)
-    witness ( (x: K, xs: seq<K>) => None)
-
-  /**   For some reasons the following lemma cannot be proved. */
-  lemma {:axiom} Foo101<K(!new)>(f: WellDefined<K>)
-    ensures forall x: K, xs: seq<K> :: f(x, xs).Some? ==> f(x, xs).v in xs
-  //   {
-  //     assume forall x: K, xs: seq<K> :: f(x, xs).Some? ==> f(x, xs).v in xs;
-  //   }
-
-  lemma {:axiom} Foo102<K(!new)>(f: WellDefined2<K>)
-    ensures forall x: K, xs: seq<K> :: f(x, xs).Some? ==> f(x, xs).v < |xs|
-    {}
-  //   {
-  //     assume forall x: K, xs: seq<K> :: f(x, xs).Some? ==> f(x, xs).v in xs;
-  //   }
+  import opened AutomataV2
 
   /**
     *   History of the DFS.
@@ -222,7 +118,7 @@ module DFSSimple {
     * @returns          The automaton and the history of visited nodes.
     */
   method DFS<T(!new)>(
-    g: Graph<T>,
+    succ: T -> seq<T>,
     s: T,
     history: History<T>,
     a: Auto<T>,
@@ -245,17 +141,17 @@ module DFSSimple {
       // DFS from s
       h' := history;
       a' := a;
-      for i := 0 to |g.succ(s)|
+      for i := 0 to |succ(s)|
         invariant a'.IsValid()
         invariant h'.IsValid()
         invariant |h'.path| == |history.path|
       {
-        print "Unfolding ", s, " -> ", g.succ(s)[i], "\n";
-        var n := h'.IsCovered(g.succ(s)[i]);
+        print "Unfolding ", s, " -> ", succ(s)[i], "\n"; 
+        var n := h'.IsCovered(succ(s)[i]);
         if n.None? {
-          var h1 := h'.AddToPathHistory(i, g.succ(s)[i]);
-          //   print "a' = ", a'.addEdge(s, g.succ(s)[i]), "\n";
-          a', h' := DFS(g, g.succ(s)[i], h1, a'.addEdge(s, g.succ(s)[i]), maxDepth - 1);
+          var h1 := h'.AddToPathHistory(i, succ(s)[i]);
+          //   print "a' = ", a'.addEdge(s, succ(s)[i]), "\n";
+          a', h' := DFS(succ, succ(s)[i], h1, a'.addEdge(s, succ(s)[i]), maxDepth - 1);
           h' := h'.PathHistoryInit();
           print a', "\n";
         } else {
