src/dafny/utils/AutomataV2.dfy
@@ -1,0 +1,120 @@
+/*
+ * Copyright 2023 Franck Cassez
+ *
+ * Licensed under the Apache License, Version 2.0 (the "License"); you may
+ * not use this file except in compliance with the License. You may obtain
+ * a copy of the License at http://www.apache.org/licenses/LICENSE-2.0
+ *
+ * Unless required by applicable law or agreed to in writing, software dis-
+ * tributed under the License is distributed on an "AS IS" BASIS, WITHOUT
+ * WARRANTIES OR CONDITIONS OF ANY KIND, either express or implied. See the
+ * License for the specific language governing permissions and limitations
+ * under the License.
+ */
+
+include "./MiscTypes.dfy"
+include "../utils/int.dfy"
+
+/** 
+  * Provides finite automata.
+  */
+module AutomataV2 { 
+
+  import opened MiscTypes
+  import opened Int
+
+  /**
+    *  Automaton.
+    *  @param toString     The string representation of a state.
+    *  @param transitions  The transition function.
+    *  @param states       The set of states.
+    *  @note               A valid automaton is such that every state has an entry in the transitions map.
+    *                      If the state has no successor then the entry is the empty list.
+    */
+  datatype Auto<!T(!new,==)> = Auto(toString: T -> string, transitions: map<T, seq<T>> := map[], states: seq<T> := [])
+  {
+    function addEdge(i: T, j: T): (a: Auto<T>)
+      requires IsValid()
+      ensures a.IsValid()
+    {
+      if i in transitions then
+        if j in transitions[i] then
+          this
+        else
+          this
+          .(transitions := transitions[i := transitions[i] + [j]] + (if j !in states then map[j := []] else map[]))
+          .(states  := states + (if j in states then [] else [j]))
+      else
+        this
+        .(transitions := transitions + map[i := [j]] + map[j := []])
+        .(states := states + [i, j])
+    }
+
+    /**
+      * Returns the number of states of the automaton.
+      */
+    function SSize(): nat
+      requires this.IsValid()
+    {
+      |states|
+    }
+
+    /** Number of transitions of the automaton. */
+    function TSize(xd: seq<T> := states): nat
+      requires this.IsValid()
+      requires (forall i : T :: i in xd ==> i in transitions)
+    {
+      if xd == [] then 0
+      else
+        assert xd[0] in states;
+        |transitions[xd[0]]| + TSize(xd[1..])
+    }
+
+    /** 
+      *  Successors of a state.
+      *  @param s  The state.
+      */
+    function Succ(s: T): seq<T>
+      requires this.IsValid()
+      requires s in states
+    {
+      transitions[s]
+    }
+
+    /**
+      * String representation of a state.
+      */
+    function ToString(t: T): string {
+      toString(t)
+    }
+
+    /** Print to Dot format. */
+    method {:print} ToDot()
+      requires this.IsValid()
+    {
+      print "digraph G {\n";
+      print "// Number of states: ", NatToString(SSize()), "\n";
+      print "// Number of transitions : ", NatToString(TSize()), "\n";
+      for i := 0 to |states| {
+        print ToString(states[i]) + ";\n";
+      }
+      for i := 0 to |states| {
+        for j := 0 to |Succ(states[i])| {
+          print ToString(states[i]) + " -> " + ToString(transitions[states[i]][j]) +
+                "[label=\"" + NatToString(j) + "\"]"
+                + ";\n";
+        }
+      }
+      print "}\n";
+    }
+
+    /** 
+      *  Check that the automaton is well formed.
+      *  @note   A well-formed automaton is such that every state has an entry in the transitions map.
+      *          If the state has no successor then the entry is the empty list.
+      */
+    ghost predicate IsValid() {
+      && (forall i : T :: i in states <==> i in transitions)
+    }
+  }
+}
